WIP to get bitvectors explecitly, probably not worth it...

SSA/Examples/InstCombine.lean
@@ -1,40 +1,156 @@
 import SSA.WellTypedFramework
+import Aesop
 
 namespace InstCombine
 
--- TODO: base these on the actual arith dialect and the target rewrite(s)
-inductive BaseType
-  | BitVector (width : Nat)
+inductive LengthIndexedList (α : Type u) : Nat → Type u where
+   | nil : LengthIndexedList α 0
+   | cons : α → LengthIndexedList α n → LengthIndexedList α (n + 1)
   deriving Repr, DecidableEq
+
+def LengthIndexedList.fromList {α : Type u} (l : List α) : LengthIndexedList α (List.length l) :=
+  match l with
+  | [] => LengthIndexedList.nil
+  | x :: xs => LengthIndexedList.cons x (LengthIndexedList.fromList xs)
+
+@[simp]
+def LengthIndexedList.foldl {α β : Type u} {n : Nat} (f : β → α → β) (acc : β) : LengthIndexedList α n → β
+  | nil => acc
+  | cons x xs => LengthIndexedList.foldl f (f acc x) xs
+
+@[simp]
+def LengthIndexedList.zipWith {α β γ : Type u} {n : Nat} (f : α → β → γ) :
+    LengthIndexedList α n → LengthIndexedList β n → LengthIndexedList γ n
+  | nil, nil => nil
+  | cons x xs, cons y ys => cons (f x y) (zipWith f xs ys)
+
+abbrev Width := Nat
+--
+structure BitVector (width : Width) where
+  (bits : LengthIndexedList Bool width)
+  deriving Repr, DecidableEq
+
+def nextSignificantBit (val : Nat) (b : Bool) := 2 * val + if (b = true) then 1 else 0
+
+-- We could instead just define this directly as Fin (2^width)
+def RawBitVectorVal {w : Width} (x : LengthIndexedList Bool w) : Nat :=
+  x.foldl nextSignificantBit 0
+
+-- #eval RawBitVectorVal (LengthIndexedList.fromList [false,true]) -- 1
+-- #eval RawBitVectorVal (LengthIndexedList.fromList [true,false,false,false]) -- 8
+-- #eval RawBitVectorVal $ LengthIndexedList.fromList [true,true,false,false,false] -- 24
+-- #eval RawBitVectorVal $ LengthIndexedList.fromList [true,false,false,false, true] -- 17
+#eval RawBitVectorVal $ (LengthIndexedList.fromList [true,false,false,false]).cons true -- 24
+
+theorem nextSignificantBitTrue {val : Nat} : nextSignificantBit val true = 2 * val + 1 := by
+  simp [nextSignificantBit]
+
+theorem nextSignificantBitFalse {val : Nat} : nextSignificantBit val false = 2 * val := by
+  simp [nextSignificantBit]
+
+theorem RawBitVectorFalse {w : Width} {x : LengthIndexedList Bool w} :
+  (LengthIndexedList.cons false x).foldl nextSignificantBit 0 = x.foldl nextSignificantBit 0 := by simp[LengthIndexedList.foldl, nextSignificantBitFalse]
+
+def testExample := fun n => [true,false,true].foldl nextSignificantBit n
+#eval [0,1,2,3,4,5].map testExample
+theorem foldNextSignificantBit {w : Nat} {x : LengthIndexedList Bool w} {v : Nat} :
+  x.foldl nextSignificantBit n = 2^w + x.foldl nextSignificantBit 0 := by
+    induction x with
+      | nil => simp[LengthIndexedList.foldl, nextSignificantBit]
+      | cons b bs ih => simp
+
+
+
+theorem RawBitVectorValNil : RawBitVectorVal (LengthIndexedList.nil) = 0 := by
+  simp [RawBitVectorVal]
+
+-- Appends to the most significant bit
+theorem RawBitVectorValConsTrue {w : Width} (x : LengthIndexedList Bool w) (b : Bool) :
+    RawBitVectorVal (x.cons true) =  2 * RawBitVectorVal x + 1 := by
+      simp [RawBitVectorVal, LengthIndexedList.foldl]
+      rw [LengthIndexedList.foldl]
+
+
+
+theorem RawBitVectorValGrowth {w : Width} (x : LengthIndexedList Bool (w - 1)) : ∀ b : Bool, RawBitVectorVal (x.cons b) ≤ 2 * RawBitVectorVal x := by
+  intro b; cases b with
+   | false => simp [RawBitVectorVal]; rw [Nat.two_mul]
+              apply Nat.le_add_left
+   | true => simp [RawBitVectorVal]; unfold LengthIndexedList.foldl <;> cases w
+
+
+theorem BitVector.valRawLT {w : Width} (x : LengthIndexedList Bool w) : RawBitVectorVal x < 2^w := by
+  simp [RawBitVectorVal]
+  induction x with
+  | nil => simp
+  | cons b bs ih => cases b with
+    | false => rw [Nat.pow_succ,Nat.mul_two]
+               apply Nat.lt_add_right
+               simp [LengthIndexedList.foldl] at *
+               exact ih
+    | true => simp  [LengthIndexedList.foldl] at *
+
+
+def BitVector.val {w : Width} (x : BitVector w) : Fin (2^w) :=
+
+
+inductive BaseType
+  | bitvec (w : Width) : BaseType
 
 instance : Goedel BaseType where
   toType := fun
-    | BaseType.BitVector _ => List Bool
+    | .bitvec w => BitVector w
 
 abbrev UserType := SSA.UserType BaseType
 
 -- See: https://releases.llvm.org/14.0.0/docs/LangRef.html#bitwise-binary-operations
 inductive Op
-  | and
-  | or
-  | xor
-  | shr
-  | lshr
-  | ashr
+  | and (w : Width) : Op
+  | or (w : Width) : Op
+  | xor (w : Width) : Op
+  | shr (w : Width) : Op
+  | lshr (w : Width) : Op
+  | ashr (w : Width) : Op
   deriving Repr, DecidableEq
 
-def argKind : Op → UserType := sorry
+-- Can we get rid of the code repetition here? (not that copilot has any trouble completing this)
+def argUserType : Op → UserType
+  | Op.and w => .pair (.base (BaseType.bitvec w)) (.base (BaseType.bitvec w))
+  | Op.or w => .pair (.base (BaseType.bitvec w)) (.base (BaseType.bitvec w))
+  | Op.xor w => .pair (.base (BaseType.bitvec w)) (.base (BaseType.bitvec w))
+  | Op.shr w => .pair (.base (BaseType.bitvec w)) (.base (BaseType.bitvec w))
+  | Op.lshr w => .pair (.base (BaseType.bitvec w)) (.base (BaseType.bitvec w))
+  | Op.ashr w => .pair (.base (BaseType.bitvec w)) (.base (BaseType.bitvec w))
+
+def outUserType : Op → UserType
+  | Op.and w => .base (BaseType.bitvec w)
+  | Op.or w => .base (BaseType.bitvec w)
+  | Op.xor w => .base (BaseType.bitvec w)
+  | Op.shr w => .base (BaseType.bitvec w)
+  | Op.lshr w => .base (BaseType.bitvec w)
+  | Op.ashr w => .base (BaseType.bitvec w)
+
 def rgnDom : Op → UserType := sorry
 def rgnCod : Op → UserType := sorry
-def outKind : Op → UserType := sorry
-def eval : ∀ (o : Op), Goedel.toType (argKind o) → (Goedel.toType (rgnDom o) →
-    Goedel.toType (rgnCod o)) → Goedel.toType (outKind o) := sorry
+
+def BitVector.bitWiseOp : ∀ {w : Width}, (Bool → Bool → Bool) → BitVector w → BitVector w → BitVector w
+  | _, f, {val := x}, {val := y} => {val := LengthIndexedList.zipWith (fun a b => f a b) x y}
+
+def BitVector.and : ∀ {w : Width}, BitVector w → BitVector w → BitVector w := BitVector.bitWiseOp (· && ·)
+def BitVector.or : ∀ {w : Width}, BitVector w → BitVector w → BitVector w := BitVector.bitWiseOp (· || ·)
+def BitVector.xor : ∀ {w : Width}, BitVector w → BitVector w → BitVector w := BitVector.bitWiseOp (fun a b => (a || b) && (¬ a || ¬ b))
+
+-- op1 * 2op2 mod 2n, where n is the width of the result
+def eval : ∀ (o : Op), Goedel.toType (argUserType o) → (Goedel.toType (rgnDom o) →
+    Goedel.toType (rgnCod o)) → Goedel.toType (outUserType o) :=
+    fun o arg _ => match o, arg with
+      | Op.and w, .pair x y => fun (x y : BitVector w) => .base {val := (LengthIndexedList.zipWith (fun a b => a && b) x.val y.val)}
 
 instance : SSA.TypedUserSemantics Op BaseType where
-  argKind := argKind
+  argUserType := argUserType
   rgnDom := rgnDom
   rgnCod := rgnCod
-  outKind := outKind
+  outUserType := outUserType
   eval := eval
 
 end InstCombine
